Common/StateT.v
@@ -4,54 +4,42 @@ Require Import CBase.
 Require Import Options.
 Require Import Effects.
 
-Module ST.
-  Section ST.
-    Context {S : Type}.
-    Context `{MRet M} `{MBind M} `{MJoin M} `{FMap M}.
+Section ST.
+  Context {St : Type}.
+  Context `{MRet M} `{MBind M} `{MJoin M} `{FMap M}.
 
-    Definition t (A : Type):= S → M (S * A).
+  Definition stateT (A : Type):= St → M (St * A).
 
-    Definition lift {A : Type} (m : M A) : ST.t A := λ s, fmap (s,.) m.
+  Definition st_lift {A : Type} (m : M A) : stateT A := λ s, fmap (s,.) m.
 
-    (** Accessors fora accesing fields of a record like state *)
-    Definition get {T} (proj : S → T)  : t T := λ s, mret (s, proj s).
-    Definition set {T} (proj : S → T) {st : Setter proj} (f : T → T) : t () :=
-      λ s, mret (set proj f s, ()).
-    Definition setv {T} (proj : S → T) {st : Setter proj} (f : T) : t () :=
-      λ s, mret (setv proj f s, ()).
+  #[global] Instance st_ret : MRet stateT := λ _ a s, mret (s, a).
+  #[global] Instance st_bind : MBind stateT := λ _ _ f ma s,
+      '(s', a) ← ma s; f a s'.
+  #[global] Instance st_join : MJoin stateT := λ _ mma s, '(s', y) ← mma s; y s'.
+  #[global] Instance st_fmap : FMap stateT := λ _ _ f ma s,
+      (ma s) |$> (λ '(s, a), (s, f a)).
 
-    (** Accessors for getting the whole state *)
-    Definition geta : t S := fun s => mret (s, s).
-    Definition seta (f : S → S) : t () := fun s => mret (f s, ()).
-    Definition setav (s : S) : t () := fun _ => mret (s, ()).
+  #[global] Instance st_call_MState : MCall (MState St) stateT | 10 := λ _ eff,
+      match eff with
+      | MSet s => λ _, mret (s, ())
+      | MGet => λ s, mret (s, s)
+      end.
 
-    Global Instance mret_inst : MRet t :=
-      { mret _ a := fun s => mret (s, a) }.
-    Global Instance mbind_inst : MBind t :=
-      { mbind _ _ f x := fun s => '(s', a) ← x s; f a s'}.
-    Global Instance mjoin_inst : MJoin t :=
-      { mjoin _ x := fun s => '(s', y) ← x s; y s'}.
-    Global Instance fmap_inst : FMap t :=
-      { fmap _ _ f x := fun s => fmap (fun '(s, a) => (s, f a)) (x s)}.
+  #[global] Instance st_throw `{MThrow E M}: MThrow E stateT :=
+    λ _ x, st_lift (mthrow x).
 
-    Context `{MThrow E M}.
-    Global Instance mthrow_inst : MThrow E t :=
-      { mthrow _ x := lift (mthrow x) }.
-
-    (* Specific instance can override this if they want the effect to modify the
-    state, but they probably shouldn't *)
-    Context `{MCall Eff M}.
-    Global Instance mcall_inst : MCall Eff t :=
-     { mcall _ eff := lift (mcall eff) }.
-
-
-  End ST.
-  Arguments t : clear implicits.
-
-  Definition move {S M M' A} (f : M (S * A)%type → M'(S * A)%type) (x : t S M A)
-      : t S M' A :=
-    fun s => f (x s).
-
-
+  (* Specific instances can override this if they want a state modifying effect
+  different from MState. *)
+  #[global] Instance st_call_inner `{MCall Eff M} : MCall Eff stateT | 100 :=
+    λ _ eff, st_lift (mcall eff).
 
 End ST.
+Arguments stateT : clear implicits.
+
+(** Move to a state transformer monad over a different monad *)
+Definition st_move {St M M' A} (f : M (St * A)%type → M' (St * A)%type)
+    (mx : stateT St M A) : stateT St M' A :=
+  λ s, f (mx s).
+
+(** The state monad is just the state transformer over the id monad *)
+Notation stateM St := (stateT St idM).
