promising-arm/UMPromising.v
@@ -485,7 +485,7 @@ End IIS.
 
 (** Runs an outcome. *)
 Definition run_outcome (tid : nat) (initmem : memoryMap) A (o : outcome A) :
-   ST.t (TState.t * Memory.t * IIS.t) (Exec.t string) A := λ '(ts, mem, iis),
+   stateT (TState.t * Memory.t * IIS.t) (Exec.t string) A := λ '(ts, mem, iis),
   let initmem := Memory.initial_from_memMap initmem in
   let deps_to_view :=
     λ deps, IIS.from_DepOn deps ts.(TState.regs) iis in
